secure_api/merkle_tree/MerkleTree.Bug.fst
@@ -1,0 +1,24 @@
+module MerkleTree.Bug
+
+open FStar.Integers
+
+module V = LowStar.Vector
+module B = LowStar.Buffer
+module HST = FStar.HyperStack.ST
+
+type hash_size_t = n:V.uint32_t{n > 0ul}
+type hash (#hsz:hash_size_t) = b:B.buffer FStar.UInt8.t { B.len b = hsz \/ B.g_is_null b }
+
+let f (#hsz:hash_size_t) (h:hash #hsz)
+: HST.ST (V.vector (hash #hsz))
+    (requires (fun h0 -> True))
+    (ensures (fun h0 v h1 -> True))
+= let v = V.alloc_empty hash in
+  let h0 = HST.get() in
+  assert (V.live h0 v);
+  assume (V.freeable v);
+  assert (not (V.is_full v));
+  assume (HST.is_eternal_region (V.frameOf v));
+  assert (V.Vec?.sz v == 0ul);
+  assert (V.Vec?.cap v == 0ul);
+  V.insert v h
